{
 "cells": [
  {
   "cell_type": "markdown",
   "metadata": {},
   "source": [
    "# Chapter 7 Conceptual Exercises"
   ]
  },
  {
   "cell_type": "markdown",
   "metadata": {},
   "source": [
    "## Problem 1\n",
    "\n",
    "$$f(x) = \\beta_0 + \\beta_1 x + \\beta_2 x^2 + \\beta_3 x^3 + \\beta_4 (x-\\xi)^3_+$$\n",
    "\n",
    "Where $(x-\\xi)^3_+ = (x-\\xi)^3$ if $x>\\xi$, and 0 otherwise.\n",
    "\n",
    "a) $$f_1(x) = a_1 + b_1 x + c_1 x^2 + d_1 x^3$$\n",
    "\n",
    "For $x \\le \\xi$, the term with $\\beta_4$ is equal to zero.\n",
    "\n",
    "$$f(x) = f_1(x)$$\n",
    "\n",
    "$$\\beta_0 + \\beta_1 x + \\beta_2 x^2 + \\beta_3 x^3 = a_1 + b_1 x + c_1 x^2 + d_1 x^3$$\n",
    "\n",
    "Then, in order for both functions to be equal, the coefficient of terms with the same exponent in $x$ must be equal:\n",
    "\n",
    "$$a_1 = \\beta_0$$\n",
    "$$b_1 = \\beta_1$$\n",
    "$$c_1 = \\beta_2$$\n",
    "$$d_1 = \\beta_3$$\n",
    "\n",
    "b) $$f_2(x) = a_2 + b_2 x + c_2 x^2 + d_2 x^3$$\n",
    "\n",
    "For $x \\gt \\xi$:\n",
    "\n",
    "$$f(x) = f_2(x)$$\n",
    "\n",
    "$$\\beta_0 + \\beta_1 x + \\beta_2 x^2 + \\beta_3 x^3 + \\beta_4 (x-\\xi)^3 = a_2 + b_2 x + c_2 x^2 + d_2 x^3$$\n",
    "\n",
    "The cubic term $(x-\\xi)^3$ can be expanded using the formula:\n",
    "\n",
    "$$(a-b)^3 = a^3 - 3a^2 b + 3ab^2 - b^3$$\n",
    "\n",
    "Then:\n",
    "\n",
    "$$\\beta_4(x-\\xi)^3 = \\beta_4x^3 - 3\\beta_4x^2\\xi + 3\\beta_4x\\xi^2 - \\beta_4\\xi^3$$\n",
    "\n",
    "Putting it all together:\n",
    "\n",
    "$$\\beta_0 + \\beta_1 x + \\beta_2 x^2 + \\beta_3 x^3 + \\beta_4x^3 - 3\\beta_4x^2\\xi + 3\\beta_4x\\xi^2 - \\beta_4\\xi^3 = a_2 + b_2 x + c_2 x^2 + d_2 x^3$$\n",
    "\n",
    "The left-hand side can be rearranged, grouping terms with the same power of $x$:\n",
    "\n",
    "$$\\beta_0 - \\beta_4\\xi^3 + \\beta_1 x + 3\\beta_4x\\xi^2 + \\beta_2 x^2 - 3\\beta_4x^2\\xi + \\beta_3 x^3 + \\beta_4x^3 = a_2 + b_2 x + c_2 x^2 + d_2 x^3$$\n",
    "\n",
    "$$\\beta_0 - \\beta_4\\xi^3 + (\\beta_1 + 3\\beta_4\\xi^2)x + (\\beta_2 - 3\\beta_4\\xi)x^2 + (\\beta_3 + \\beta_4)x^3 = a_2 + b_2 x + c_2 x^2 + d_2 x^3$$\n",
    "\n",
    "Now we can equate coefficients with the same power of $x$:\n",
    "\n",
    "$$a_2 = \\beta_0 - \\beta_4\\xi^3$$\n",
    "$$b_2 = \\beta_1 + 3\\beta_4\\xi^2$$\n",
    "$$c_2 = \\beta_2 - 3\\beta_4\\xi$$\n",
    "$$d_2 = \\beta_3 + \\beta_4$$\n",
    "\n",
    "c) $$f_1(\\xi) = a_1 + b_1 \\xi + c_1 \\xi^2 + d_1 \\xi^3$$\n",
    "\n",
    "$$\\boxed{f_1(\\xi) = \\beta_0 + \\beta_1 \\xi + \\beta_2 \\xi^2 + \\beta_3 \\xi^3}$$\n",
    "\n",
    "$$f_2(\\xi) = a_2 + b_2 \\xi + c_2 \\xi^2 + d_2 \\xi^3$$\n",
    "\n",
    "$$f_2(\\xi) = \\beta_0 - \\beta_4\\xi^3 + (\\beta_1 + 3\\beta_4\\xi^2) \\xi + (\\beta_2 - 3\\beta_4\\xi) \\xi^2 + (\\beta_3 + \\beta_4) \\xi^3$$\n",
    "\n",
    "Expanding terms for $f_2(\\xi)$:\n",
    "\n",
    "$$f_2(\\xi) = \\beta_0 - \\cancel{\\beta_4\\xi^3} + \\beta_1\\xi + \\cancel{3\\beta_4\\xi^3} + \\beta_2\\xi^2 - \\cancel{3\\beta_4\\xi^3} + \\beta_3\\xi^3 + \\cancel{\\beta_4\\xi^3}$$\n",
    "\n",
    "After cancelling terms:\n",
    "\n",
    "$$\\boxed{f_2(\\xi) = \\beta_0 + \\beta_1 \\xi + \\beta_2 \\xi^2 + \\beta_3 \\xi^3}$$\n",
    "\n",
    "Then, $f(x)$ is continuous at $\\xi$:\n",
    "\n",
    "$$\\boxed{f_1(\\xi) = f_2(\\xi)}$$\n",
    "\n",
    "d) If $f(x) = a + b x + c x^2 + d x^3$, then the derivative is $f'(x) = b + 2c x + 3d x^2$. Then:\n",
    "\n",
    "$$f_1'(\\xi) = b_1 + 2c_1 \\xi + 3d_1 \\xi^2$$\n",
    "$$f_2'(\\xi) = b_2 + 2c_2 \\xi + 3d_2 \\xi^2$$\n",
    "\n",
    "Rewriting in terms of betas:\n",
    "\n",
    "$$f_1'(\\xi) = \\beta_1 + 2\\beta_2 \\xi + 3\\beta_3 \\xi^2$$\n",
    "$$f_2'(\\xi) = \\beta_1 + 3\\beta_4\\xi^2 + 2 (\\beta_2 - 3\\beta_4\\xi) \\xi + 3 (\\beta_3 + \\beta_4) \\xi^2$$\n",
    "\n",
    "Expanding terms for $f_2'(\\xi)$:\n",
    "\n",
    "$$f_2'(\\xi) = \\beta_1 + 3\\beta_4\\xi^2 + 2 \\beta_2 \\xi - 6\\beta_4\\xi^2 + 3 \\beta_3 \\xi^2 + 3\\beta_4 \\xi^2$$\n",
    "\n",
    "Cancelling terms:\n",
    "\n",
    "$$f_2'(\\xi) = \\beta_1 + 2 \\beta_2 \\xi + 3 \\beta_3 \\xi^2$$\n",
    "\n",
    "Then:\n",
    "\n",
    "$$\\boxed{f_1'(\\xi) = f_2'(\\xi)}$$\n",
    "\n",
    "e) The second derivative is $f''(x) = 2c + 6dx$. Then:\n",
    "\n",
    "$$f_1''(\\xi) = 2c_1 + 6d_1\\xi$$\n",
    "$$f_2''(\\xi) = 2c_2 + 6d_2\\xi$$\n",
    "\n",
    "Rewriting in terms of betas:\n",
    "\n",
    "$$f_1''(\\xi) = 2\\beta_2 + 6\\beta_3\\xi$$\n",
    "$$f_2''(\\xi) = 2(\\beta_2 - 3\\beta_4\\xi) + 6(\\beta_3 + \\beta_4)\\xi$$\n",
    "\n",
    "Expanding terms for $f_2''(\\xi)$:\n",
    "\n",
    "$$f_2''(\\xi) = 2\\beta_2 - 6\\beta_4\\xi + 6\\beta_3\\xi + 6\\beta_4\\xi$$\n",
    "\n",
    "Cancelling terms:\n",
    "\n",
    "$$f_2''(\\xi) = 2\\beta_2 + 6\\beta_3\\xi$$\n",
    "\n",
    "Then:\n",
    "\n",
    "$$\\boxed{f_1''(\\xi) = f_2''(\\xi)}$$"
   ]
  },
  {
   "cell_type": "markdown",
   "metadata": {},
   "source": []
  }
 ],
 "metadata": {
  "kernelspec": {
   "display_name": "venv",
   "language": "python",
   "name": "python3"
  },
  "language_info": {
   "name": "python",
   "version": "3.11.2"
  }
 },
 "nbformat": 4,
 "nbformat_minor": 2
}
